src/lang/Thread.v
@@ -137,7 +137,7 @@ Module Thread.
     Definition consistent (e:t): Prop :=
       forall mem1 sc1
         (CAP: Memory.cap e.(local).(Local.promises) e.(memory) mem1)
-        (SC_FUTURE: Memory.max_full_timemap mem1 sc1),
+        (SC_MAX: Memory.max_full_timemap mem1 sc1),
       exists e2,
         <<STEPS: rtc tau_step (mk e.(state) e.(local) sc1 mem1) e2>> /\
         <<PROMISES: e2.(local).(Local.promises) = Memory.bot>>.
